porting the tacticals.

theories/RTac/Apply.v
@@ -6,6 +6,7 @@ Require Import MirrorCore.LemmaApply.
 Require Import MirrorCore.InstantiateI.
 Require Import MirrorCore.RTac.Core.
 Require Import MirrorCore.RTac.Reduce.
+Require Import MirrorCore.RTac.EApply.
 
 Require Import MirrorCore.Util.Forwardy.
 
@@ -26,36 +27,29 @@ Section parameterized.
   Context {SubstUpdateOk_subst : @SubstUpdateOk _ _ _ _ Expr_expr Subst_subst _ _}.
 
   Variable vars_to_uvars : nat -> nat -> expr -> expr.
-  Variable exprUnify :
+  Variable exprUnify : forall subst, Subst subst expr -> SubstUpdate subst expr ->
     tenv typ -> tenv typ -> nat -> expr -> expr -> typ -> subst -> option subst.
   Variable instantiate : (nat -> option expr) -> nat -> expr -> expr.
   Variable UVar : nat -> expr.
 
-  Let eapplicable :=
-    @eapplicable typ _ expr _ subst vars_to_uvars
-                 exprUnify.
+  Variable lem : Lemma.lemma typ expr expr.
 
-  Definition APPLY
-             (lem : Lemma.lemma typ expr expr)
-  : rtac typ expr subst :=
-    let len_vars := length lem.(vars) in
-    fun ctx sub goal =>
-      let '(tus,tvs) := getEnvs ctx in
-      match eapplicable sub tus tvs lem goal with
-        | None => Fail
-        | Some sub' =>
-          let len_uvars := length tus in
-          match pull (expr := expr) (SU := SU) len_uvars len_vars sub' with
-            | Some sub'' =>
-              let premises :=
-                  map (fun e => instantiate (fun u => lookup u sub') 0
-                                            (vars_to_uvars 0 len_uvars e))
-                      lem.(premises)
-              in
-              more_list instantiate UVar CTop sub'' (map GGoal premises)
-              (** Solve the side conditions **)
-            | None => Fail
-          end
-      end.
+  Definition APPLY : rtac typ expr subst :=
+    @EAPPLY typ expr subst _ _ _ _ vars_to_uvars exprUnify lem.
+  Let tyProp := @typ0 _ _ Prop _.
+
+  Let cast (e : typD tyProp) : Prop :=
+    match @typ0_cast typ _ Prop _ in _ = T return T with
+      | eq_refl => e
+    end.
+
+  Hypothesis lemD :
+    @Lemma.lemmaD typ _ expr _ expr (@exprD'_typ0 _ _ _ _ Prop _)
+                  tyProp cast nil nil lem.
+
+  Theorem APPLY_sound : rtac_sound nil nil APPLY.
+  Proof.
+    eapply EAPPLY_sound.
+  Qed.
 
 End parameterized.
