theories/RTac/EApply.v
@@ -1,10 +1,9 @@
 Require Import ExtLib.Structures.Monad.
 Require Import ExtLib.Tactics.
-Require Import MirrorCore.ExprI.
-Require Import MirrorCore.SubstI.
 Require Import MirrorCore.ExprDAs.
 Require Import MirrorCore.Lemma.
 Require Import MirrorCore.LemmaApply.
+Require Import MirrorCore.InstantiateI.
 Require Import MirrorCore.RTac.Core.
 Require Import MirrorCore.RTac.Reduce.
 
@@ -27,21 +26,22 @@ Section parameterized.
   Context {SubstUpdateOk_subst : @SubstUpdateOk _ _ _ _ Expr_expr Subst_subst _ _}.
 
   Variable vars_to_uvars : nat -> nat -> expr -> expr.
-  Variable exprUnify : tenv typ -> tenv typ -> nat -> expr -> expr -> typ -> subst -> option subst.
+  Variable exprUnify : forall subst, Subst subst expr -> SubstUpdate subst expr ->
+    tenv typ -> tenv typ -> nat -> expr -> expr -> typ -> subst -> option subst.
   Variable instantiate : (nat -> option expr) -> nat -> expr -> expr.
   Variable UVar : nat -> expr.
 
-  Let eapplicable :=
-    @eapplicable typ _ expr _ subst vars_to_uvars
-                 exprUnify.
+  Variable lem : Lemma.lemma typ expr expr.
 
-  Definition EAPPLY
-             (lem : Lemma.lemma typ expr expr)
-  : rtac typ expr subst :=
+  Definition EAPPLY : rtac typ expr subst :=
     let len_vars := length lem.(vars) in
-    fun ctx sub gl =>
-      let '(tus,tvs) := getEnvs ctx in
-      match eapplicable sub tus tvs lem gl with
+    fun tus tvs nus nvs ctx sub goal =>
+      match @eapplicable typ _ expr _
+                         (ctx_subst subst (CExs ctx lem.(vars)))
+                         vars_to_uvars (@exprUnify _ _ _)
+                         (@ExsSubst _ _ _ lem.(vars) ctx sub (@empty _ _ _))
+                         tus tvs lem goal
+      with
         | None => Fail
         | Some sub' =>
           let len_uvars := length tus in
@@ -49,5 +49,20 @@ Section parameterized.
           reduceGoal instantiate UVar (fold_left (@CEx _ _) lem.(vars) CTop) sub'
                      (GConj premises) (countUVars ctx + len_vars) (countVars ctx)
       end.
+
+  Let tyProp := @typ0 _ _ Prop _.
+
+  Let cast (e : typD tyProp) : Prop :=
+    match @typ0_cast typ _ Prop _ in _ = T return T with
+      | eq_refl => e
+    end.
+
+  Hypothesis lemD :
+    @Lemma.lemmaD typ _ expr _ expr (@exprD'_typ0 _ _ _ _ Prop _)
+                  tyProp cast nil nil lem.
+
+  Theorem EAPPLY_sound : rtac_sound nil nil EAPPLY.
+  Proof.
+  Admitted.
 
 End parameterized.
