theories/RTac/RunSTac.v
@@ -29,8 +29,11 @@ Section parameterized.
   Variable instantiate : (nat -> option expr) -> nat -> expr -> expr.
   Variable UVar : nat -> expr.
 
-  Definition STAC_no_hyps (tac : STac.Core.stac typ expr subst)
-  : rtac typ expr subst :=
+  Variable tac : forall subst, STac.Core.stac typ expr subst.
+
+  Definition STAC_no_hyps : rtac typ expr subst.
+red.
+  refine (
     fun tus tvs _ _ ctx sub gl =>
       match tac tus tvs sub nil gl with
         | STac.Core.Fail => Fail
@@ -44,7 +47,7 @@ Section parameterized.
                      (List.fold_right (fun x y => @CEx _ _ y x)
                        (List.fold_right (fun x y => @CAll _ _ y x)
                           CTop tvs') tus') sub' GSolved (length tus + length tus') (length tvs + length tvs')
-      end.
+      end).
 
 (*
   Lemma goalD_fold_right_GExs
